---
layout: post
title: كسور مستمرة (جذر 2)
tag: جبر
---

![Euler identity.png](/images/Euler identity.png){: style="float: center; 
height: 85%; width: 85%; margin-left: 1em; margin-top: 2em;"}{:class="img-responsive"}

<br>

لدينا

<br>

$$
\begin{split}
(\sqrt{2}-1)(\sqrt{2}+1)&=\sqrt{2}^2-1^2\\
&=2-1\\
&=1
\end{split}
$$

<br>

 و عليه
<br>

$$
\sqrt{2}-1=\frac{1}{1+\sqrt{2}}
$$

<br>

و هذا ينتج

<br>

$$
\color{blue}{\sqrt{2}=1+\frac{1}{1+\sqrt{2}}}
$$

<br>

و هذا يعطي

$$
\begin{split}
\sqrt{2}&=1+\frac{1}{1+\color{blue}{\sqrt{2}}}\\
&=\cfrac{1}{1+\color{blue}{1+\frac{1}{1+\sqrt{2}}}}
\end{split}
$$





